New combinators for oracle syntax properties
Introduce combinators is_state_oracle and oracle_monotonic.

is_state_oracle: an oracle's config values (states) are what you'd
get by repeatedly applying the incremental compiler.

oracle_monotonic: some projection of an oracle's values increases
monotonically in some order.

The first is used to make invariant-style reasoning local. We prove
the invariant on the state in the proof about the phase, and just
export the requirement that the config values that will be passed
back in via the oracle are the ones we'd expect.

The monotonic one is for ALL_DISTINCT style proofs across various
generations. All the names from install-generation 2 should be greater
than any in the previous generation.

compiler/backend/proofs/clos_knownProofScript.sml
@@ -1600,6 +1600,39 @@ Theorem oracle_gapprox_disjoint_lemma
    (rw [] \\ imp_res_tac evaluate_IMP_shift_seq
    \\ metis_tac [oracle_gapprox_disjoint_shift_seq_unique_set_globals]);
 
+val is_state_oracle_def = Define`
+  is_state_oracle compile_inc_f co init_state =
+    ((FST (FST (co 0)) = init_state) /\ (!n. FST (FST (co (SUC n)))
+        = FST (compile_inc_f (FST (FST (co n))) (SND (co n)))))`;
+
+Theorem is_state_oracle_shift:
+  is_state_oracle compile_inc_f co st =
+  (FST (FST (co 0)) = st /\ is_state_oracle compile_inc_f (shift_seq 1 co)
+        (FST (compile_inc_f st (SND (co 0)))))
+Proof
+  fs [is_state_oracle_def, shift_seq_def]
+  \\ EQ_TAC \\ rw [] \\ fs [sptreeTheory.ADD_1_SUC]
+  \\ full_simp_tac bool_ss [arithmeticTheory.ONE]
+  \\ Cases_on `n`
+  \\ fs []
+QED
+
+val oracle_monotonic_def = Define`
+  oracle_monotonic (f : 'a -> 'b set) (R : 'b -> 'b -> bool) (S : 'b set)
+    (orac : num -> 'a) =
+    ((!i j x y. i < j /\ x IN f (orac i) /\ y IN f (orac j) ==> R x y)
+        /\ (! i x y. x IN S /\ y IN f (orac i) ==> R x y))`;
+
+val conjs = MATCH_MP quotientTheory.EQ_IMPLIES (SPEC_ALL oracle_monotonic_def)
+  |> UNDISCH_ALL |> CONJUNCTS |> map DISCH_ALL
+
+Theorem oracle_monotonic_step = hd conjs;
+Theorem oracle_monotonic_init = hd (tl conjs);
+
+val compile_inc_def = Define `
+  compile_inc c g (es,xs) =
+    let (eas, g') = known (reset_inline_factor c) es [] g in (g', MAP FST eas, xs)`;
+
 val say = say0 "known_correct_approx";
 
 Theorem known_correct_approx
@@ -2105,6 +2138,86 @@ Theorem known_correct_approx
     \\ irule EVERY2_APPEND_suff \\ simp []
     \\ fs [case_eq_thms] \\ rveq \\ simp [LIST_REL_GENLIST]));
 
+Theorem monotonic_gapprox_disjoint:
+  known c xs aenv LN = (ys, g) ==>
+  oracle_monotonic (SET_OF_BAG o elist_globals o FST o SND)
+      (<) (SET_OF_BAG b) co ==>
+  b = elist_globals xs ==>
+  oracle_gapprox_disjoint g co
+Proof
+  fs [oracle_gapprox_disjoint_def]
+  \\ rw []
+  \\ first_x_assum (ASSUME_TAC o Q.SPEC `n` o HO_MATCH_MP oracle_monotonic_init)
+  \\ imp_res_tac known_changed_globals
+  \\ rw [gapprox_disjoint_def, pred_setTheory.IN_DISJOINT]
+  \\ fs []
+  \\ metis_tac [prim_recTheory.LESS_REFL]
+QED
+
+Theorem elist_globals_FLAT_APPEND_FOLDR:
+  elist_globals (xs ++ FLAT ys) = FOLDR $⊎ {||} (MAP elist_globals (xs :: ys))
+Proof
+  Induct_on `ys`
+  \\ fs [elist_globals_append, ASSOC_BAG_UNION]
+QED
+
+Theorem elist_globals_FLAT_FOLDR = (Q.INST [`xs` |-> `[]`]
+    elist_globals_FLAT_APPEND_FOLDR |> SIMP_RULE list_ss []);
+
+Theorem monotonic_unique_set_globals:
+  oracle_monotonic (SET_OF_BAG o elist_globals o FST o SND) (<)
+      (SET_OF_BAG (elist_globals xs)) co ==>
+  BAG_ALL_DISTINCT (elist_globals xs) /\
+  (!n. BAG_ALL_DISTINCT (elist_globals (FST (SND (co n))))) ==>
+  unique_set_globals xs co
+Proof
+  rw [unique_set_globals_def, elist_globals_FLAT_APPEND_FOLDR]
+  \\ fs [BAG_ALL_DISTINCT_BAG_UNION, BAG_ALL_DISTINCT_FOLDR_BAG_UNION,
+    BAG_DISJOINT_FOLDR_BAG_UNION, first_n_exps_def, EL_MAP]
+  \\ rw []
+  >- (
+    rw [BAG_DISJOINT_BAG_IN]
+    \\ drule oracle_monotonic_step
+    \\ fs []
+    \\ metis_tac [prim_recTheory.LESS_REFL]
+  )
+  \\ rw [EVERY_EL, EL_MAP, BAG_DISJOINT_BAG_IN]
+  \\ drule oracle_monotonic_init
+  \\ fs []
+  \\ metis_tac [prim_recTheory.LESS_REFL]
+QED
+
+Theorem pure_co_oracle_props:
+  oracle_gapprox_subspt (pure_co f ∘ co) = oracle_gapprox_subspt co /\
+  oracle_state_sgc_free (pure_co f ∘ co) = oracle_state_sgc_free co
+Proof
+  fs [oracle_gapprox_subspt_def, oracle_state_sgc_free_def]
+QED
+
+Theorem state_oracle_domain:
+  is_state_oracle (compile_inc c) co g ==>
+  BAG_OF_SET (domain (FST (FST (co n)))) <= BAG_UNION
+    (BAG_OF_SET (domain g)) (elist_globals (FLAT (first_n_exps co n)))
+Proof
+  rw []
+  \\ Induct_on `n` \\ fs [is_state_oracle_def]
+  \\ Cases_on `SND (co n)` \\ fs [compile_inc_def]
+  \\ pairarg_tac \\ fs []
+  \\ drule known_changed_globals_alt
+  \\ fs [first_n_exps_def, GENLIST, FLAT_SNOC, elist_globals_append]
+  \\ rw []
+  \\ irule SUB_BAG_TRANS
+  \\ goal_assum drule
+  \\ metis_tac [SUB_BAG_UNION_eliminate, ASSOC_BAG_UNION]
+QED
+
+(* FIXME: move *)
+Theorem DISJOINT_BAG_DISJOINT:
+  DISJOINT (SET_OF_BAG b) (SET_OF_BAG b') ==> BAG_DISJOINT b b'
+Proof
+  fs [BAG_DISJOINT]
+QED
+
 (* code relation *)
 
 val exp_rel_def = Define `
@@ -2286,10 +2399,6 @@ val ref_rel_simps = save_thm("ref_rel_simps[simp]",LIST_CONJ [
 Theorem ref_rel_upd_inline_factor
   `ref_rel (c with inline_factor := k) = ref_rel c`
   (simp [FUN_EQ_THM, ref_rel_cases, v_rel_upd_inline_factor]);
-
-val compile_inc_def = Define `
-  compile_inc c g (es,xs) =
-    let (eas, g') = known (reset_inline_factor c) es [] g in (g', MAP FST eas, xs)`;
 
 val state_rel_def = Define `
   state_rel c g (s:(val_approx num_map#'c,'ffi) closSem$state) (t:('c,'ffi) closSem$state) <=>
@@ -4291,19 +4400,29 @@ Theorem compile_LENGTH
 
 val syntax_ok_def = Define`
   syntax_ok xs ⇔
-    every_Fn_vs_NONE xs ∧
+    every_Fn_vs_NONE xs /\
+    BAG_ALL_DISTINCT (elist_globals xs) /\
     EVERY esgc_free xs`;
 
+val _ = temp_overload_on("fvs_compile",``clos_fvs$compile``);
+
+val fvs_inc_def = Define`
+  (fvs_inc : exp list # 'a list -> exp list # 'a list)
+    = clos_fvsProof$compile_inc`;
+
+Theorem fvs_inc_unfold:
+  fvs_inc x = (remove_fvs 0 (FST x), [])
+Proof
+  Cases_on `x` \\ EVAL_TAC
+QED
+
 val syntax_oracle_ok_def = Define`
-  syntax_oracle_ok xs co ⇔
-    syntax_ok xs ∧
-    co_every_Fn_vs_NONE co ∧
-    oracle_state_sgc_free co ∧
-    oracle_gapprox_subspt co ∧
-    oracle_gapprox_disjoint (FST (FST (co 0))) co ∧
-    unique_set_globals xs co ∧
-    (∀n. SND(SND(co n)) = [] ∧
-         syntax_ok (FST (SND (co n))))`;
+  syntax_oracle_ok c xs co conf ⇔
+    syntax_ok xs /\
+    is_state_oracle (compile_inc c) (pure_co fvs_inc o co) conf /\
+    oracle_monotonic (SET_OF_BAG o elist_globals o FST o SND) (<)
+      (SET_OF_BAG (elist_globals xs)) co /\
+    (!n. syntax_ok (FST (SND (co n))) /\ SND (SND (co n)) = [])`
 
 val known_cc_def = Define `
   known_cc known_conf cc =
@@ -4331,18 +4450,88 @@ Theorem FST_known_co
   (rw[known_co_def] \\ CASE_TAC
   \\ simp[backendPropsTheory.FST_state_co]);
 
+Theorem syntax_oracle_ok_state_sgc_free:
+  syntax_oracle_ok c xs co g ==>
+  known c (fvs_compile xs) [] LN = (ys, g) ==>
+  oracle_state_sgc_free co
+Proof
+  fs [oracle_state_sgc_free_def, syntax_oracle_ok_def]
+  \\ rw []
+  \\ Induct_on `n`
+  >- (
+    fs [is_state_oracle_def, clos_fvsTheory.compile_def]
+    \\ drule known_preserves_esgc_free
+    \\ fs [syntax_ok_def]
+    \\ impl_tac \\ fs []
+    \\ fs [globals_approx_sgc_free_def, lookup_def]
+  )
+  \\ fs [is_state_oracle_def, fvs_inc_unfold]
+  \\ Cases_on `SND (co n)` \\ fs [compile_inc_def]
+  \\ pairarg_tac \\ fs []
+  \\ drule (Q.SPEC `reset_inline_factor foo` known_preserves_esgc_free)
+  \\ impl_tac \\ fs []
+  \\ fs [PAIR_FST_SND_EQ] \\ rveq
+  \\ fs [syntax_ok_def, clos_fvsTheory.compile_def]
+QED
+
+Theorem syntax_oracle_ok_gapprox_subspt:
+  syntax_oracle_ok c xs co g ==>
+  known c (fvs_compile xs) [] LN = (ys, g) ==>
+  oracle_gapprox_subspt co
+Proof
+  rw []
+  \\ imp_res_tac (GEN_ALL syntax_oracle_ok_state_sgc_free)
+  \\ fs [oracle_gapprox_subspt_def, syntax_oracle_ok_def]
+  \\ imp_res_tac state_oracle_domain
+  \\ drule monotonic_unique_set_globals
+  \\ impl_tac >- fs [syntax_ok_def]
+  \\ fs []
+  \\ imp_res_tac monotonic_gapprox_disjoint
+  \\ fs [is_state_oracle_def]
+  \\ rw []
+  \\ Cases_on `SND (co n)` \\ fs [fvs_inc_unfold, compile_inc_def]
+  \\ pairarg_tac \\ fs []
+  \\ drule (Q.SPECL [`c`, `xs`, `[]`] known_subspt)
+  \\ fs [clos_fvsTheory.compile_def]
+  \\ impl_tac \\ fs []
+  \\ fs [BAG_ALL_DISTINCT_BAG_UNION]
+  \\ fs [oracle_gapprox_disjoint_def, gapprox_disjoint_def]
+  \\ rpt (first_x_assum (assume_tac o Q.SPEC `n`))
+  \\ rfs []
+  \\ fs [syntax_ok_def, oracle_state_sgc_free_def]
+  \\ drule BAG_DISJOINT_SUB_BAG
+  \\ disch_then irule
+  \\ fs [unique_set_globals_def]
+  \\ fs [PAIR_FST_SND_EQ] \\ rveq
+  \\ fs [DISJOINT_BAG_DISJOINT]
+  \\ rpt (first_x_assum (assume_tac o Q.SPEC `SUC n`))
+  \\ fs [first_n_exps_def, GENLIST, FLAT_SNOC, elist_globals_append,
+        BAG_ALL_DISTINCT_BAG_UNION]
+  \\ fs [elist_globals_FLAT_FOLDR, MAP_GENLIST, o_DEF, fvs_inc_unfold]
+QED
+
+Theorem oracle_monotonic_subset:
+  ((St' SUBSET St) /\ (!n. f' (co' n) SUBSET f (co n))) ==>
+  oracle_monotonic f R St co ==>
+  oracle_monotonic f' R St' co'
+Proof
+  fs [oracle_monotonic_def, SUBSET_DEF]
+  \\ metis_tac []
+QED
+
 Theorem semantics_compile
   `closSem$semantics ffi max_app FEMPTY co cc1 xs ≠ Fail ∧
    (cc1 = known_cc known_conf cc) ∧
    (co1 = known_co known_conf co) ∧
    (compile known_conf xs = (known_conf', es)) ∧
    (IS_SOME known_conf ⇒
-      syntax_oracle_ok xs co ∧ 1 ≤ max_app ∧
-      FST (FST (co 0)) = (THE known_conf').val_approx_spt)
+      syntax_oracle_ok (THE known_conf) xs co (THE known_conf').val_approx_spt ∧
+      1 ≤ max_app)
    ⇒
    semantics ffi max_app FEMPTY co1 cc es =
    semantics ffi max_app FEMPTY co cc1 xs`
-  (simp [known_co_def,known_cc_def]
+  (
+  simp [known_co_def,known_cc_def]
   \\ strip_tac
   \\ Cases_on`known_conf` \\ fs[compile_def]
   >- ( match_mp_tac semantics_CURRY_I \\ fs[] )
@@ -4352,8 +4541,10 @@ Theorem semantics_compile
   >- ( fs[syntax_oracle_ok_def] )
   \\ disch_then (fn th => fs [GSYM th])
   \\ drule (GEN_ALL semantics_known) \\ fs []
-  \\ impl_keep_tac THEN1
-   (fs[syntax_ok_def,syntax_oracle_ok_def]
+  \\ impl_keep_tac THEN1 (
+    imp_res_tac syntax_oracle_ok_gapprox_subspt
+    \\ imp_res_tac syntax_oracle_ok_state_sgc_free
+    \\ fs[syntax_ok_def,syntax_oracle_ok_def]
     \\ simp[clos_fvsTheory.compile_def]
     \\ conj_tac
     >- ( gen_tac \\ Cases_on`SND (co n)` \\ EVAL_TAC )
@@ -4379,35 +4570,22 @@ Theorem semantics_compile
       \\ rw[] \\ rw[]
       \\ first_x_assum(qspec_then`n`mp_tac)
       \\ rw[] )
-    \\ fs[oracle_gapprox_subspt_def]
-    \\ fs[oracle_state_sgc_free_def]
+    \\ fs[pure_co_oracle_props]
     \\ conj_tac
     >- (
-      fs[unique_set_globals_def, elist_globals_append, first_n_exps_def]
-      \\ fs[elist_globals_FOLDR, MAP_FLAT, MAP_GENLIST]
-      \\ fs[o_DEF]
-      \\ gen_tac
-      \\ qmatch_goalsub_abbrev_tac`FLAT (GENLIST X n)`
-      \\ qmatch_asmsub_abbrev_tac`GENLIST Y`
-      \\ `X =Y`
-      by (
-        simp[Abbr`X`,Abbr`Y`, FUN_EQ_THM]
-        \\ qx_gen_tac`m` \\ Cases_on`SND (co m)` \\ EVAL_TAC
-        \\ simp[])
-      \\ fs[] )
-    \\ fs[oracle_gapprox_disjoint_def]
+      irule monotonic_unique_set_globals
+      \\ fs [syntax_ok_def, GSYM fvs_inc_def, fvs_inc_unfold, o_DEF]
+      \\ first_assum (fn t => mp_tac t \\ match_mp_tac oracle_monotonic_subset)
+      \\ fs [fvs_inc_unfold])
     \\ conj_tac
     >- (
       drule clos_fvsProofTheory.fv_max_remove_fvs
       \\ disch_then(qspec_then`0`mp_tac)
       \\ rw[fv_max_def] )
-    \\ fs[gapprox_disjoint_def]
-    \\ gen_tac
-    \\ Cases_on`SND (co n)`
-    \\ simp[clos_fvsProofTheory.compile_inc_def]
-    \\ first_x_assum(qspec_then`n`mp_tac) \\ simp[]
-    \\ first_x_assum(qspec_then`n`mp_tac) \\ simp[]
-    \\ simp[clos_fvsTheory.compile_def] )
+    \\ imp_res_tac monotonic_gapprox_disjoint
+    \\ fs [clos_fvsTheory.compile_def]
+    \\ fs[oracle_gapprox_disjoint_def, gapprox_disjoint_def, GSYM fvs_inc_def, fvs_inc_unfold, is_state_oracle_def]
+  )
   \\ disch_then (fn th => fs [GSYM th])
   \\ drule (GEN_ALL clos_ticksProofTheory.semantics_remove_ticks)
   \\ impl_keep_tac THEN1
